Prove Lemma 34 using Lemma 31 (sorry)

Isabelle/Inspector.thy
@@ -150,7 +150,9 @@ lemma (in Protocol) validator_in_clique_see_L_H_M_of_others_is_singleton :
   \<longrightarrow> (\<forall> v v'. {v, v'} \<subseteq> v_set \<longrightarrow> is_singleton (L_H_M (the_elem (L_H_J \<sigma> v)) v'))"
   sorry
 
+(* ###################################################### *)
 (* Section 7.3: Cliques Survive Messages from Validators Outside Clique *)
+(* ###################################################### *)
 
 (* Lemma 11: Minimal transitions do not change Later_From for any non-sender *)
 lemma (in Protocol) later_from_of_non_sender_not_affected_by_minimal_transitions :
@@ -309,7 +311,10 @@ lemma (in Protocol) new_message_from_majority_clique_see_members_agreeing :
   \<longrightarrow> sender m' \<in> agreeing_validators (p, justification m')"
   oops
 
+
+(* ###################################################### *)
 (* 7.4.4 Honest messages from majority clique members do not break the clique *)
+(* ###################################################### *)
 
 (* Lemma 25 *)
 lemma (in Protocol) latest_message_in_justification_of_new_message_is_latest_message :
@@ -318,7 +323,6 @@ lemma (in Protocol) latest_message_in_justification_of_new_message_is_latest_mes
   \<longrightarrow> sender m' \<notin> equivocating_validators \<sigma>'
   \<longrightarrow> the_elem (L_H_M (justification m') (sender m')) = the_elem (L_H_M \<sigma> (sender m'))"
   oops
-
 
 (* Lemma 26 *)
 lemma (in Protocol) latest_message_justified_by_new_message :
@@ -361,17 +365,19 @@ lemma (in Protocol) empty_later_disagreeing_messages_in_new_message :
   oops
 
 (* Lemma 31 (New non-equivocating latest messages from members of majority clique don’t break the clique) *)
-lemma (in Protocol) clique_not_affected_by_minimal_transitions_outside_clique :
-  "\<forall> \<sigma> \<sigma>' m' v_set p. (\<sigma>, \<sigma>') \<in> minimal_transitions \<and> v_set \<subseteq> V 
+lemma (in Protocol) clique_not_affected_by_honest_message_from_member :
+  "\<forall> \<sigma> m v_set p. \<sigma> \<in> \<Sigma>t \<and> m \<in> M \<and> v_set \<subseteq> V 
   \<longrightarrow> majority_driven p
-  \<longrightarrow> m' = the_elem (\<sigma>' - \<sigma>)
-  \<longrightarrow> is_clique (v_set, p, \<sigma>) \<and> sender m' \<in> v_set \<and> sender m' \<notin> equivocating_validators \<sigma>'
-      \<and> (\<forall> v \<in> v_set. majority (v_set, the_elem (L_H_J \<sigma> v))) 
-  \<longrightarrow> is_clique (v_set, p, \<sigma>')"
-  oops
+  \<longrightarrow> immediately_next_message (\<sigma>, m)
+  \<longrightarrow> sender m \<in> v_set
+  \<longrightarrow> \<not> is_equivocating (\<sigma> \<union> {m}) (sender m)
+  \<longrightarrow> is_clique (v_set, p, \<sigma>) 
+  \<longrightarrow> is_clique (v_set, p, \<sigma> \<union> {m})"
+  sorry
 
-
+(* ###################################################### *)
 (* 7.5 Equivocations from Validators in Clique do not break cliques *)
+(* ###################################################### *)
 
 (* Definition 7.18: One layer clique oracle threshold size *) 
 definition (in Params) gt_threshold :: "(validator set * state) \<Rightarrow> bool"
@@ -387,10 +393,12 @@ lemma (in Protocol) gt_threshold_imps_majority_for_any_validator :
   oops
 
 (* Definition 7.19: Clique oracle with 1 layers *)
+(* FIXME: Make the order of variables consistent to is_clique *)
+(* Removed "- E(\<sigma>)" part from the original definition since it is included in is_clique *)
 definition (in Params) is_clique_oracle :: "(validator set * state * consensus_value_property) \<Rightarrow> bool"
   where
     "is_clique_oracle 
-       = (\<lambda>(v_set, \<sigma>, p). (is_clique (v_set - (equivocating_validators \<sigma>), p, \<sigma>) \<and> gt_threshold (v_set - (equivocating_validators \<sigma>), \<sigma>)))"
+       = (\<lambda>(v_set, \<sigma>, p). (is_clique (v_set, p, \<sigma>) \<and> gt_threshold (v_set, \<sigma>)))"
 
 (* Lemma 33: Clique oracles preserved over message from non-member *)
 lemma (in Protocol) clique_oracles_preserved_over_message_from_non_member :
@@ -411,7 +419,10 @@ lemma (in Protocol) clique_oracles_preserved_over_message_from_non_equivocating_
   \<longrightarrow> \<not> is_equivocating (\<sigma> \<union> {m}) (sender m)
   \<longrightarrow> is_clique_oracle (v_set, \<sigma>, p) 
   \<longrightarrow> is_clique_oracle (v_set, \<sigma> \<union> {m}, p)"
-  sorry
+  using clique_not_affected_by_honest_message_from_member
+  unfolding is_clique_oracle_def gt_threshold_def
+  using equivocating_validators_preserved_over_honest_message
+  using \<Sigma>t_is_subset_of_\<Sigma> by auto
 
 (* Lemma 35: Clique oracles preserved over message from equivocating member *)
 lemma (in Protocol) clique_oracles_preserved_over_message_from_equivocating_member :
@@ -423,6 +434,7 @@ lemma (in Protocol) clique_oracles_preserved_over_message_from_equivocating_memb
   \<longrightarrow> \<sigma> \<union> {m} \<in> \<Sigma>t
   \<longrightarrow> is_clique_oracle (v_set, \<sigma>, p) 
   \<longrightarrow> is_clique_oracle (v_set, \<sigma> \<union> {m}, p)"
+  (* using free_sub_clique *)
   sorry
 
 
