Isabelle/CBCCasper.thy
@@ -337,6 +337,13 @@ lemma (in Protocol) equivocation_is_monotonic :
   apply (simp add: equivocating_validators_def is_equivocating_def)
   using observed_def by fastforce
 
+lemma (in Protocol) equivocating_validators_preserved_over_honest_message :
+  "\<forall> \<sigma> m. \<sigma> \<in> \<Sigma> \<and> m \<in> M
+  \<longrightarrow> \<not> is_equivocating (\<sigma> \<union> {m}) (sender m)
+  \<longrightarrow> equivocating_validators \<sigma> = equivocating_validators (\<sigma> \<union> {m})"
+  apply (simp add: equivocating_validators_def is_equivocating_def observed_def equivocation_def)
+  by auto
+  
 (* ###################################################### *)
 (* Weight measure *)
 (* ###################################################### *)
